src/ConcurrentSemantics.v
@@ -1,5 +1,6 @@
 (* This part of the work is based on https://dl.acm.org/doi/10.1145/3123569.3123576 *)
 Require Export SubstSemantics.
+Require Export Coq.Sorting.Permutation.
 
 Import ListNotations.
 
@@ -10,6 +11,8 @@ Inductive Action : Set :=
 | ASend (p : PID) (t : Exp)
 | AReceive (t : Exp)
 | AArrive (t : Exp)
+| ASelf (ι : PID)
+| ASpawn (ι : PID) (t1 t2 : Exp)
 | AInternal.
 
 Fixpoint find_clause (v : Exp) (c : list (Pat * Exp)) : option (Exp * list Exp) :=
@@ -32,6 +35,26 @@ end.
 
 Definition pop (v : Exp) (m : Mailbox) := remove Exp_eq_dec v m.
 
+Fixpoint len (l : Exp) : option nat :=
+match l with
+| ENil => Some 0
+| VCons v1 v2 => match len v2 with
+                 | Some n2 => Some (S n2)
+                 | _ => None
+                 end
+| _ => None
+end.
+
+Fixpoint mk_list (l : Exp) : option (list Exp) :=
+match l with
+| ENil => Some []
+| VCons v1 v2 => match mk_list v2 with
+                 | Some l => Some (v1 :: l)
+                 | _ => None
+                 end
+| _ => None
+end.
+
 Reserved Notation "p -⌈ a ⌉-> p'" (at level 50).
 Inductive processLocalSemantics : Process -> Action -> Process -> Prop :=
 | p_local fs e fs' e' mb :
@@ -43,12 +66,24 @@ Inductive processLocalSemantics : Process -> Action -> Process -> Prop :=
   (fs, ESend ι e, mb) -⌈ AInternal ⌉-> (FSend1 e :: fs, ι, mb)
 | p_send_local2 fs e v mb : VALCLOSED v ->
   (FSend1 e :: fs, v, mb) -⌈ AInternal ⌉-> (FSend2 v :: fs, e, mb)
+| p_spawn_local1 fs e ι mb :
+  (fs, ESpawn ι e, mb) -⌈ AInternal ⌉-> (FSpawn1 e :: fs, ι, mb)
+| p_spawn_local2 fs e v mb : VALCLOSED v ->
+  (FSpawn1 e :: fs, v, mb) -⌈ AInternal ⌉-> (FSpawn2 v :: fs, e, mb)
+
 
 | p_arrive mb mb' fs e v : VALCLOSED v -> mb' = mb ++ [v] ->
   (fs, e, mb) -⌈ AArrive v ⌉-> (fs, e, mb')
 
 | p_send ι v mb fs : 
   (FSend2 (EPid ι) :: fs, v, mb) -⌈ ASend ι v ⌉-> (fs, v, mb)
+
+| p_self ι fs mb :
+  ( fs, ESelf, mb ) -⌈ ASelf ι ⌉-> ( fs, EPid ι, mb )
+
+| p_spawn ι fs mb vl e l:
+  Some (length vl) = len l ->
+  (FSpawn2 (EFun vl e) :: fs, l, mb) -⌈ASpawn ι (EFun vl e) l⌉-> (fs, EPid ι, mb)
 
 | p_receive mb l fs e m mb' bindings :
   receive mb l = Some (m, e, bindings) -> mb' = pop m mb
@@ -71,53 +106,79 @@ Notation "x -⌈ k | xs ⌉-> y" := (LabelStar processLocalSemantics x k xs y) (
 Require Import Coq.Structures.OrderedTypeEx.
 
 Module Import NatMap := FMapList.Make(Nat_as_OT). *)
-From stdpp Require Import natmap fin_maps.
+(* From stdpp Require Import natmap fin_maps. *)
 
-Definition Node := natmap Process. Search natmap.
-Definition nullnode : Node := empty.
-Definition par (pid : PID) (proc: Process) (n : Node) : Node := map_insert pid proc n.
+Definition Node : Set := list (PID * Process).
+Fixpoint put (k : PID) (p : Process) (m : Node) : Node :=
+match m with
+| [] => [(k, p)]
+| (k', p')::xs => if Nat.ltb k k' then (k, p) :: (k', p') :: xs else if Nat.eqb k k' then (k, p)::xs else (k', p') :: (put k p xs)
+end.
+Fixpoint get (k : PID) (m : Node) : option Process :=
+match m with
+| [] => None
+| (k', p)::xs => if Nat.eqb k k' then Some p else get k xs
+end.
+Definition dom (m : Node) : list nat := map fst m.
 
-Notation "pid : p |||| n" := (par pid p n) (at level 30, right associativity).
+(* Definition Node := natmap Process. Search natmap. *)
+Definition nullnode : Node := [].
+(* Definition par (pid : PID) (proc: Process) (n : Node) : Node := map_insert pid proc n. *)
 
-Definition find (x : PID) (Π : Node) : option Process := lookup x Π.
+Notation "pid : p |||| n" := (put pid p n) (at level 30, right associativity).
+
+(* Definition find (x : PID) (Π : Node) : option Process := lookup x Π. *)
 
 Reserved Notation "n -[ a | ι ]ₙ-> n'" (at level 50).
 Inductive nodeSemantics : Node -> Action -> PID -> Node -> Prop :=
 | nsend1 p p' q q' Π Π' (ι ι' : PID) t :
-  find ι Π = Some p -> find ι' Π = Some q ->
+  get ι Π = Some p -> get ι' Π = Some q ->
   Π' = ι : p' |||| ι' : q' |||| Π ->
   p -⌈ASend ι' t⌉-> p' -> q -⌈AArrive t⌉-> q' -> ι <> ι'
 ->
   Π -[ASend ι' t | ι]ₙ-> Π'
 
 | nsend2 p p' p'' t (ι : PID) Π Π' :
-  find ι Π = Some p -> Π' = ι : p'' |||| Π ->
+  get ι Π = Some p -> Π' = ι : p'' |||| Π ->
   p -⌈ASend ι t⌉-> p' -> p' -⌈AArrive t⌉-> p'' (** two transitions, because this is atomic! *)
 ->
   Π -[ASend ι t | ι]ₙ-> Π'
 
 | nsend3 p p' (ι ι' : PID) Π Π' t :
-  find ι Π = Some p -> find ι' Π = None ->
+  get ι Π = Some p -> get ι' Π = None ->
   Π' = ι : p' |||| Π ->
   p -⌈ASend ι' t⌉-> p'
 ->
   Π -[ASend ι' t | ι]ₙ-> Π'
 
 | nreceive p p' t Π Π' (ι : PID) :
-  find ι Π = Some p -> Π' = ι : p' |||| Π ->
+  get ι Π = Some p -> Π' = ι : p' |||| Π ->
   p -⌈AReceive t⌉-> p'
 ->
   Π -[AReceive t | ι]ₙ-> Π'
 
 | ninternal p p' Π Π' (ι : PID) :
-  find ι Π = Some p -> Π' = ι : p' |||| Π ->
+  get ι Π = Some p -> Π' = ι : p' |||| Π ->
   p -⌈AInternal⌉-> p'
 ->
   Π -[AInternal | ι]ₙ-> Π'
 
+| nself p p' Π Π' ι:
+  get ι Π = Some p -> Π' = ι : p' |||| Π ->
+  p -⌈ASelf ι⌉-> p'
+->
+  Π -[ASelf ι | ι]ₙ-> Π'
+
+| nspawn Π Π' p p' v1 v2 l ι ι':
+  mk_list v2 = Some l -> ~In ι' (dom Π) ->
+  get ι Π = Some p -> Π' = ι' : ([], EApp v1 l, []) |||| ι : p' |||| Π ->
+  p -⌈ASpawn ι' v1 v2⌉-> p'
+->
+  Π -[ASpawn ι' v1 v2 | ι]ₙ-> Π'
 where "n -[ a | ι ]ₙ-> n'" := (nodeSemantics n a ι n').
 
-(* Fixpoint Pat_eqb (p1 p2 : Pat) : bool :=
+(*
+Fixpoint Pat_eqb (p1 p2 : Pat) : bool :=
 match p1, p2 with
  | PLit l, PLit l2 => Z.eqb l l2
  | PPid p, PPid p2 => p =? p2
@@ -136,13 +197,13 @@ end.
 
 Fixpoint Exp_eqb (e1 e2 : Exp) : bool :=
 match e1, e2 with
- | ELit l, ELit l2 => Z.eqb l =? l2
+ | ELit l, ELit l2 => Z.eqb l l2
  | EPid p, EPid p2 => p =? p2
  | EVar n, EVar n2 => n =? n2
  | EFunId n, EFunId n2 => n =? n2
  | EFun vl e, EFun vl2 e2 => list_eqb String.eqb vl vl2 && Exp_eqb e e2
- | EApp exp l, EApp exp2 l2 => Exp_eqb exp exp2 && list_eqb Exp_eqb
- | ELet v e1 e2, ELet v2 e12 e22 => _
+ | EApp exp l, EApp exp2 l2 => Exp_eqb exp exp2 && list_eqb Exp_eqb l l2
+ | ELet v e1 e2, ELet v2 e12 e22 => Exp_eqb e1 e12 && Exp_eqb e12 e22
  | ELetRec f vl b e, ELetRec f2 vl2 b2 e2 => _
  | EPlus e1 e2, EPlus e12 e22 => _
  | ECase e0 p e1 e2, ECase e02 p2 e12 e22 => _
@@ -165,17 +226,27 @@ match n1 with
 | {| this := x; sorted := y |} => length n2 = length x /\ list_eq_Node x n2
 end. *)
 
-#[export] Instance processEq : Equiv Process := eq.
+(* #[export] Instance processEq : Equiv Process := eq. *)
 
 Reserved Notation "n -[ k | l ]ₙ->* n'" (at level 50).
 Inductive closureNodeSem : Node -> nat -> list (Action * PID) -> Node -> Prop :=
-| nrefl n n' : map_equiv n n' -> n -[ 0 | [] ]ₙ->* n'
+| nrefl n (* n'  *): (* Permutation n n' -> *) n -[ 0 | [] ]ₙ->* n (* ' *)
 | ntrans n n' n'' k l a ι:
   n -[a|ι]ₙ-> n' -> n' -[k|l]ₙ->* n''
 ->
   n -[S k | (a,ι)::l]ₙ->* n''
 where "n -[ k | l ]ₙ->* n'" := (closureNodeSem n k l n').
 
+Ltac perm_solver :=
+match goal with
+| |- Permutation [] [] => apply perm_nil
+| |- Permutation (_::_) (_::_) =>
+  tryif apply perm_skip
+  then  (idtac "ok")
+  else  (idtac "move"; eapply perm_trans; [apply Permutation_cons_append | simpl] )
+| _ => idtac "not permutation goal"
+end.
+Ltac perm_solver_any := repeat perm_solver.
 (*
   0 -[ 1 + 1 ]-> 1
   1 -[ 2 ]-> 3
@@ -232,7 +303,7 @@ Proof.
   constructor; try reflexivity. cbn.
   break_match_goal. 2: congruence.
   break_match_goal. 2: congruence.
-  break_match_goal. simpl in e1. inversion e1.
+  break_match_goal. congruence.
   eapply ntrans. eapply nreceive with (ι := 3); cbn; try reflexivity.
   constructor; try reflexivity.
 
@@ -243,10 +314,70 @@ Proof.
   eapply ntrans. eapply ninternal with (ι := 3); cbn; try reflexivity.
   constructor. constructor.
 
-  apply nrefl.
-  simpl. cbn.
   break_match_goal. 2: congruence.
-  cbn. intro. intros. auto.
+  apply nrefl.
+Qed.
+
+(*
+
+let X = spawn(fun() -> receive X -> X ! self() end end, [])
+  in let Y = X ! self()
+    in receive X -> X end
+
+*)
+Goal exists acts k,
+  0 : ([], ELet "X"%string (ESpawn (EFun [] (EReceive [(PVar, ESend (EVar 0) ESelf)]
+                                            )) ENil)
+             (ELet "Y"%string (ESend (EVar 0) ESelf)
+                 (EReceive [(PVar, EVar 0)]))
+                  , [])
+  
+  |||| nullnode
+  -[ k | acts ]ₙ->*
+  0 : ([], EPid 1, []) ||||
+  1 : ([], EPid 1, []) |||| nullnode.
+Proof.
+  eexists. exists 19.
+  eapply ntrans. eapply ninternal with (ι := 0); cbn; try reflexivity.
+  do 2 constructor.
+  eapply ntrans. eapply ninternal with (ι := 0); cbn; try reflexivity.
+  apply p_spawn_local1.
+  eapply ntrans. eapply ninternal with (ι := 0); cbn; try reflexivity.
+  apply p_spawn_local2. do 2 constructor. intros. inversion H; subst; cbn. 2: inversion H1. repeat constructor.
+  eapply ntrans. eapply nspawn with (ι := 0) (ι' := 1); simpl. 2: lia. 2: reflexivity.
+  3: constructor. all: simpl; auto.
+  eapply ntrans. eapply ninternal with (ι := 0); cbn; try reflexivity.
+  do 3 constructor.
+  eapply ntrans. eapply ninternal with (ι := 1); cbn; try reflexivity.
+  repeat constructor.
+  eapply ntrans. eapply ninternal with (ι := 1); cbn; try reflexivity.
+  repeat constructor. simpl.
+  eapply ntrans. eapply ninternal with (ι := 0); cbn; try reflexivity.
+  repeat constructor.
+  eapply ntrans. eapply ninternal with (ι := 0); cbn; try reflexivity.
+  apply p_send_local1.
+  eapply ntrans. eapply ninternal with (ι := 0); cbn; try reflexivity.
+  apply p_send_local2. constructor.
+  eapply ntrans. eapply nself with (ι := 0); cbn; try reflexivity.
+  constructor.
+  eapply ntrans. eapply nsend1 with (ι := 0) (ι' := 1); cbn; try reflexivity; auto.
+  constructor. constructor; auto. constructor.
+  eapply ntrans. eapply ninternal with (ι := 0); cbn; try reflexivity.
+  repeat constructor. simpl.
+  eapply ntrans. eapply nreceive with (ι := 1); cbn; try reflexivity.
+  repeat constructor. simpl. break_match_goal. 2: congruence.
+  eapply ntrans. eapply ninternal with (ι := 1); cbn; try reflexivity.
+  apply p_send_local1.
+  eapply ntrans. eapply ninternal with (ι := 1); cbn; try reflexivity.
+  apply p_send_local2. constructor.
+  eapply ntrans. eapply nself with (ι := 1); cbn; try reflexivity.
+  constructor.
+  eapply ntrans. eapply nsend1 with (ι := 1) (ι' := 0); cbn; try reflexivity; auto.
+  constructor. constructor; auto. constructor. simpl.
+  eapply ntrans. eapply nreceive with (ι := 0); simpl; try reflexivity.
+  constructor; auto. reflexivity. simpl.
+  break_match_goal. 2: congruence.
+  apply nrefl.
 Qed.
 
 Definition bisimulation (R : Node -> Node -> Prop) :=
